fix: LClass proofs finished

lean-formalisation/LeanFormalisation/LClass/LClassDefs.lean
@@ -82,7 +82,7 @@ inductive Lang : Tag → Type
 | UnOp (arg : Lang .Expr) (op : UnOp) : Lang .Expr
 | New (cls : Nat) (args : Fin n → Lang .Expr) : Lang .Expr
 | Call (m : Nat) (cls : Nat) (args : Fin n → Lang .Expr) : Lang .Expr
-| Return (l : Nat) (e : Lang .Expr) : Lang .Expr
+| Return (e : Lang .Expr) (l : Nat) : Lang .Expr
 | If (cond : Lang .Expr) (e₁ : Lang .Expr) (e₂ : Lang .Expr) : Lang .Expr
 | While (cond : Lang .Expr) (body : Lang .Expr) : Lang .Expr
 | Break (l : Nat) : Lang .Expr
@@ -109,7 +109,6 @@ notation:100 s₁:100 ";" s₂:101 => Lang.Seq s₁ s₂
 notation x "::=" exp => Lang.Assign x exp
 abbrev Ctx := List Ty
 
-abbrev JCtx := List Nat
 notation Γ₁ "("x")" "=" type => x < List.length Γ₁ ∧ Γ₁[x]? = Option.some type
 
 inductive TypR : Tag → Type
@@ -130,116 +129,116 @@ structure Defs (cCnt : Nat) where
 
 variable (cCnt : Nat) (defs : Defs cCnt)
 
+inductive JumpFrame
+| Loop (n : Nat)
+| Method (cls : Fin cCnt) (m : Fin (defs.methodsCnt cls))
+deriving Inhabited
+
+abbrev JCtx := List (JumpFrame cCnt defs)
+
+inductive LoopJump : JCtx cCnt defs → Nat → Prop
+| LoopBase (n : Nat) :
+  LoopJump (.Loop n :: Δ) 0
+| Loop (n : Nat) (l : Nat) :
+  LoopJump Δ (l - 1) →
+  LoopJump (.Loop n :: Δ) l
+
 inductive Typ :
-  (tg : Tag) → (cCur : Fin cCnt) → (Fin (defs.methodsCnt cCur)) →
-  JCtx → Ctx → Lang tg → TypR tg → Prop
+  (tg : Tag) →
+  JCtx cCnt defs → Ctx → Lang tg → TypR tg → Prop
 -- # Expr
-| TrueConst
-  (cCur : Fin cCnt) (mCur : Fin (defs.methodsCnt cCur)) :
-  Typ .Expr cCur mCur Δ₁ Γ₁ .True (.Expr .bool)
-| FalseConst
-  (cCur : Fin cCnt) (mCur : Fin (defs.methodsCnt cCur)) :
-  Typ .Expr cCur mCur Δ₁ Γ₁ .False (.Expr .bool)
+| TrueConst :
+  Typ .Expr Δ₁ Γ₁ .True (.Expr .bool)
+| FalseConst :
+  Typ .Expr Δ₁ Γ₁ .False (.Expr .bool)
 | NatConst
-  (cCur : Fin cCnt) (mCur : Fin (defs.methodsCnt cCur))
   (n : Nat) :
-  Typ .Expr cCur mCur Δ₁ Γ₁ (.Nat n) (.Expr .nat)
-| UnitConst
-  (cCur : Fin cCnt) (mCur : Fin (defs.methodsCnt cCur)) :
-  Typ .Expr cCur mCur Δ₁ Γ₁ .Unit (.Expr .unit)
+  Typ .Expr Δ₁ Γ₁ (.Nat n) (.Expr .nat)
+| UnitConst :
+  Typ .Expr Δ₁ Γ₁ .Unit (.Expr .unit)
 | VarAccess
-  (cCur : Fin cCnt) (mCur : Fin (defs.methodsCnt cCur))
   (x : VarName) (type : Ty) :
   (Γ₁(x) = type) →
-  Typ .Expr cCur mCur Δ₁ Γ₁ (.Var x) (.Expr type)
+  Typ .Expr Δ₁ Γ₁ (.Var x) (.Expr type)
 | FieldAccess
-  (cCur : Fin cCnt) (mCur : Fin (defs.methodsCnt cCur))
-  (n : Nat) (f : Nat) (p : Lang .Expr) :
+  (n : Nat) (f : Nat) (p : Lang .Expr) (ty : Ty) :
   (hn : n < cCnt) →
   (hf : f < defs.fieldsCnt ⟨n, hn⟩) →
-  Typ .Expr cCur mCur Δ₁ Γ₁ p (.Expr (.cls n)) →
-  Typ .Expr cCur mCur Δ₁ Γ₁ (.Field f p) (.Expr (defs.fieldsTy ⟨n, hn⟩ ⟨f, hf⟩))
+  Typ .Expr Δ₁ Γ₁ p (.Expr (.cls n)) →
+  ty = (defs.fieldsTy ⟨n, hn⟩ ⟨f, hf⟩) →
+  Typ .Expr Δ₁ Γ₁ (.Field f p) (.Expr ty)
 | UnOp
-  (cCur : Fin cCnt) (mCur : Fin (defs.methodsCnt cCur))
-  (arg : Lang .Expr) (op : UnOp) :
-  Typ .Expr cCur mCur Δ₁ Γ₁ arg (.Expr op.args.1) →
-  Typ .Expr cCur mCur Δ₁ Γ₁ (.UnOp arg op) (.Expr op.args.2)
+  (arg : Lang .Expr) (op : UnOp) (ty : Ty) :
+  Typ .Expr Δ₁ Γ₁ arg (.Expr op.args.1) →
+  ty = op.args.2 →
+  Typ .Expr Δ₁ Γ₁ (.UnOp arg op) (.Expr ty)
 | BinOp
-  (cCur : Fin cCnt) (mCur : Fin (defs.methodsCnt cCur))
-  (arg₁ arg₂ : Lang .Expr) (op : BinOp) :
-  Typ .Expr cCur mCur Δ₁ Γ₁ arg₁ (.Expr op.args.1) →
-  Typ .Expr cCur mCur Δ₁ Γ₁ arg₂ (.Expr op.args.2) →
-  Typ .Expr cCur mCur Δ₁ Γ₁ (.BinOp arg₁ arg₂ op) (.Expr op.args.3)
+  (arg₁ arg₂ : Lang .Expr) (op : BinOp) (ty : Ty) :
+  Typ .Expr Δ₁ Γ₁ arg₁ (.Expr op.args.1) →
+  Typ .Expr Δ₁ Γ₁ arg₂ (.Expr op.args.2) →
+  ty = op.args.3 →
+  Typ .Expr Δ₁ Γ₁ (.BinOp arg₁ arg₂ op) (.Expr ty)
 | New
-  (cCur : Fin cCnt) (mCur : Fin (defs.methodsCnt cCur))
-  (cls : Nat) (hc : cls < cCnt) (args : Fin (defs.fieldsCnt ⟨cls, hc⟩) → Lang .Expr):
-  ∀ i, Typ .Expr cCur mCur Δ₁ Γ₁ (args i) (.Expr (defs.fieldsTy ⟨cls, hc⟩ i)) →
-  Typ .Expr cCur mCur Δ₁ Γ₁ (.New cls args) (.Expr (.cls cls))
-| Call
-  (cCur : Fin cCnt) (mCur : Fin (defs.methodsCnt cCur))
   (cls : Nat) (hc : cls < cCnt)
-  (m : Nat) (hm : m < defs.methodsCnt ⟨cls, hc⟩)
-  (args : Fin (defs.methods ⟨cls, hc⟩ ⟨m, hm⟩).nArg → Lang .Expr) (ret : Ty) :
-  (defs.methods ⟨cls, hc⟩ ⟨m, hm⟩).ret = ret →
-  ∀ i, Typ .Expr cCur mCur Δ₁ Γ₁ (args i) (.Expr ((defs.methods ⟨cls, hc⟩ ⟨m, hm⟩).argTy i)) →
-  /-
-  -- well typed part
-  Typ .Expr ⟨cls, hc⟩ ⟨m, hm⟩
-    [] (List.ofFn (defs.methods ⟨cls, hc⟩ ⟨m, hm⟩).argTy)
-    (defs.methods ⟨cls, hc⟩ ⟨m, hm⟩).body (.Expr ret) →
-  -/
-  Typ .Expr cCur mCur Δ₁ Γ₁ (.Call m cls args) (.Expr ret)
-| Return (l : Nat)
-  (cCur : Fin cCnt) (mCur : Fin (defs.methodsCnt cCur))
-  (type : Ty) :
-  type = (defs.methods cCur mCur).ret →
-  Typ .Expr cCur mCur Δ₁ Γ₁ (.Return l e) (.Expr type)
+  (narg : Nat) (harg : narg = defs.fieldsCnt ⟨cls, hc⟩)
+  (args : Fin narg → Lang .Expr) :
+  (∀ i, Typ .Expr Δ₁ Γ₁ (args i) (.Expr (defs.fieldsTy ⟨cls, hc⟩ ⟨i, by omega⟩))) →
+  Typ .Expr Δ₁ Γ₁ (.New cls args) (.Expr (.cls cls))
+| Call
+  (cls : Nat) (hcls : cls < cCnt)
+  (m : Nat) (hm : m < defs.methodsCnt ⟨cls, hcls⟩)
+  (narg : Nat) (harg : (defs.methods ⟨cls, hcls⟩ ⟨m, hm⟩).nArg = narg)
+  (args : Fin narg → Lang .Expr) (ret : Ty) :
+  (defs.methods ⟨cls, hcls⟩ ⟨m, hm⟩).ret = ret →
+  (∀ i,
+    Typ .Expr Δ₁ Γ₁ (args i)
+      (.Expr ((defs.methods ⟨cls, hcls⟩ ⟨m, hm⟩).argTy ⟨i, by omega⟩))) →
+  Typ .Expr Δ₁ Γ₁ (.Call m cls args) (.Expr ret)
+| Return (e : Lang .Expr) (l : Nat) (type : Ty)
+  (cls : Fin cCnt) (m : Fin (defs.methodsCnt cls)) :
+  (hl : l < Δ₁.length) →
+  Δ₁[l]! = .Method cls m →
+  (l = 0 ∨ LoopJump cCnt defs Δ₁ (l - 1)) →
+  Typ .Expr Δ₁ Γ₁ e (.Expr (defs.methods cls m).ret) →
+  Typ .Expr Δ₁ Γ₁ (.Return e l) (.Expr type)
 | IfExpr
-  (cCur : Fin cCnt) (mCur : Fin (defs.methodsCnt cCur))
   (cond : Lang .Expr) (e₁ : Lang .Expr) (e₂ : Lang .Expr) (type : Ty) :
-  Typ .Expr cCur mCur Δ₁ Γ₁ cond (.Expr .bool) →
-  Typ .Expr cCur mCur Δ₁ Γ₁ e₁ (.Expr type) →
-  Typ .Expr cCur mCur Δ₁ Γ₁ e₂ (.Expr type) →
-  Typ .Expr cCur mCur Δ₁ Γ₁ (.If cond e₁ e₂) (.Expr type)
+  Typ .Expr Δ₁ Γ₁ cond (.Expr .bool) →
+  Typ .Expr Δ₁ Γ₁ e₁ (.Expr type) →
+  Typ .Expr Δ₁ Γ₁ e₂ (.Expr type) →
+  Typ .Expr Δ₁ Γ₁ (.If cond e₁ e₂) (.Expr type)
 | WhileExpr
-  (cCur : Fin cCnt) (mCur : Fin (defs.methodsCnt cCur))
   (cond : Lang .Expr) (body : Lang .Expr) :
-  Typ .Expr cCur mCur Δ₁ Γ₁ cond (.Expr .bool) →
-  Typ .Expr cCur mCur (Γ₁.length :: Δ₁) Γ₁ body (.Expr .unit) →
-  Typ .Expr cCur mCur Δ₁ Γ₁ (.While cond body) (.Expr .unit)
+  Typ .Expr Δ₁ Γ₁ cond (.Expr .bool) →
+  Typ .Expr (.Loop Γ₁.length :: Δ₁) Γ₁ body (.Expr .unit) →
+  Typ .Expr Δ₁ Γ₁ (.While cond body) (.Expr .unit)
 | BreakExpr
-  (cCur : Fin cCnt) (mCur : Fin (defs.methodsCnt cCur))
   (type : Ty) (l : Nat) :
-  l < Δ₁.length →
-  Typ .Expr cCur mCur Δ₁ Γ₁ (.Break l) (.Expr .unit)
+  LoopJump cCnt defs Δ₁ l →
+  Typ .Expr Δ₁ Γ₁ (.Break l) (.Expr type)
 | ScopeExpr
-  (cCur : Fin cCnt) (mCur : Fin (defs.methodsCnt cCur))
   (s : Lang .Stmt) (e : Lang .Expr) (type : Ty) :
-  Typ .Stmt cCur mCur Δ₁ Γ₁ s (.Stmt Γ₂) →
-  Typ .Expr cCur mCur Δ₁ Γ₂ e (.Expr type) →
-  Typ .Expr cCur mCur Δ₁ Γ₁ (.Scope s e) (.Expr type)
+  Typ .Stmt Δ₁ Γ₁ s (.Stmt Γ₂) →
+  Typ .Expr Δ₁ Γ₂ e (.Expr type) →
+  Typ .Expr Δ₁ Γ₁ (.Scope s e) (.Expr type)
 -- # Stmt
 | VarDecl
-  (cCur : Fin cCnt) (mCur : Fin (defs.methodsCnt cCur))
   (e : Lang .Expr) (type : Ty) :
-  Typ .Expr cCur mCur Δ₁ Γ₁ e (.Expr type) →
-  Typ .Stmt cCur mCur Δ₁ Γ₁ (.Decl type e) (.Stmt (type :: Γ₁))
+  Typ .Expr Δ₁ Γ₁ e (.Expr type) →
+  Typ .Stmt Δ₁ Γ₁ (.Decl type e) (.Stmt (type :: Γ₁))
 | VarAssign
-  (cCur : Fin cCnt) (mCur : Fin (defs.methodsCnt cCur))
   (x : VarName) (e : Lang .Expr) (type : Ty) :
-  Typ .Expr cCur mCur Δ₁ Γ₁ e (.Expr type) → (Γ₁(x) = type) →
-  Typ .Stmt cCur mCur Δ₁ Γ₁ (.Assign x e) (.Stmt Γ₁)
+  Typ .Expr Δ₁ Γ₁ e (.Expr type) → (Γ₁(x) = type) →
+  Typ .Stmt Δ₁ Γ₁ (.Assign x e) (.Stmt Γ₁)
 | Seq
-  (cCur : Fin cCnt) (mCur : Fin (defs.methodsCnt cCur))
   (s₁ s₂ : Lang .Stmt) :
-  Typ .Stmt cCur mCur Δ₁ Γ₁ s₁ (.Stmt Γ₂) →
-  Typ .Stmt cCur mCur Δ₁ Γ₂ s₂ Γ₃ →
-  Typ .Stmt cCur mCur Δ₁ Γ₁ (s₁; s₂) Γ₃
+  Typ .Stmt Δ₁ Γ₁ s₁ (.Stmt Γ₂) →
+  Typ .Stmt Δ₁ Γ₂ s₂ Γ₃ →
+  Typ .Stmt Δ₁ Γ₁ (s₁; s₂) Γ₃
 | Do
-  (cCur : Fin cCnt) (mCur : Fin (defs.methodsCnt cCur))
   (e : Lang .Expr) (type : Ty) :
-  Typ .Expr cCur mCur Δ₁ Γ₁ e (.Expr type) →
-  Typ .Stmt cCur mCur Δ₁ Γ₁ (.Do e) (.Stmt Γ₁)
+  Typ .Expr Δ₁ Γ₁ e (.Expr type) →
+  Typ .Stmt Δ₁ Γ₁ (.Do e) (.Stmt Γ₁)
 
 section TypeProperties
 
@@ -253,16 +252,13 @@ def TypR.extR (Γ₁ : Ctx) (tg : Tag) : TypR tg → TypR tg
 
 end TypeProperties
 
-def value_type : Value → Ty → Prop
-| .True, .bool => True
-| .False, .bool => True
-| .Nat _, .nat => True
-| .Unit, .unit => True
-| _, _ => False
+inductive simpleType : Value → Ty → Prop
+| True : simpleType .True .bool
+| False : simpleType .False .bool
+| Nat (n : Nat) : simpleType (.Nat n) .nat
+| Unit : simpleType .Unit .unit
 
-inductive Control
-| sourceExpr (e : Lang .Expr)
-| sourceStmt (s : Lang .Stmt)
+inductive Res
 | value (v : Value)
 | skip
 
@@ -272,17 +268,17 @@ inductive Cont
 | fieldK (f : Nat)
 | ifCondK (e₁ e₂ : Lang .Expr)
 | declK (type : Ty)
-| returnK (l : Nat)
 | assignK (x : VarName)
 | seqK (s : Lang .Stmt)
+| exprStmtK
 | binopLK (op : BinOp) (e₂ : Lang .Expr)
 | binopRK (op : BinOp) (v : Value)
 | unopK (op : UnOp)
-| loopK (c : Lang .Expr) (body : Lang .Expr) (n : Nat)
-| loopContK (c : Lang .Expr) (body : Lang .Expr) (n : Nat)
-| scopeBodyK (e : Lang .Expr) (n : Nat)
-| scopeExitK (n : Nat)
-| exprStmtK
+| loopK (c : Lang .Expr) (body : Lang .Expr)
+| loopContK (c : Lang .Expr) (body : Lang .Expr) (n : Nat) (J : List (List Cont))
+| scopeBodyK (e : Lang .Expr) (n : Nat) (J : List (List Cont))
+| scopeExitK (n : Nat) (J : List (List Cont))
+| returnJumpK (l : Nat)
 | argK (cls : Fin cCnt) (m : Fin (defs.methodsCnt cls))
   (sep : Fin (defs.methods cls m).nArg)
   (values : Fin sep → Value)
@@ -291,9 +287,13 @@ inductive Cont
   (sep : Fin (defs.fieldsCnt cls))
   (values : Fin sep → Value)
   (rems : Fin (defs.fieldsCnt cls - sep - 1) → Lang .Expr)
-| callK (E : Environment)
+| breakRestoreK (n : Nat) (J : List (List Cont))
+| returnRestoreK (E : Environment) (J : List (List Cont))
+| callRestoreK (E : Environment) (J : List (List Cont))
+deriving Inhabited
 
-abbrev JStackCtx (cCnt : Nat) (defs : Defs cCnt) := List (Nat × List (Cont cCnt defs))
+abbrev JStackCtx (cCnt : Nat) (defs : Defs cCnt) :=
+  List (List (Cont cCnt defs))
 
 variable (cCnt : Nat) (defs : Defs cCnt)
 
@@ -305,23 +305,25 @@ abbrev Map (val : Type) := Finmap (fun _ : Addr => val)
 
 abbrev Store := Map (Object cCnt defs)
 
-structure CEK where
-  C : Control
-  E : Environment
-  J : JStackCtx cCnt defs
-  S : Store cCnt defs
-  K : List (Cont cCnt defs)
--- Do we need this relation in the current Jump Context implementation?
-/-
-inductive PopLoopK : List Cont → List Cont → Nat → Prop
-| loopK (c body : Lang .Expr) (n : Nat) (rest : List Cont) :
-  PopLoopK (.loopK c body n :: rest) rest n
-| loopContK (c body : Lang .Expr) (n : Nat) (rest : List Cont) :
-  PopLoopK (.loopContK c body n :: rest) rest n
-| skip (k : Cont) (rest result : List Cont) (n : Nat) :
-  PopLoopK rest result n →
-  PopLoopK (k :: rest) result n
--/
+inductive EvalMode
+| Eval
+| Cont
+
+
+inductive CEK : EvalMode → Type
+| Eval
+  (tg : Tag)
+  (C : Lang tg)
+  (E : Environment)
+  (J : JStackCtx cCnt defs)
+  (S : Store cCnt defs)
+  (K : List (Cont cCnt defs)) : CEK .Eval
+| Cont
+  (res : Res)
+  (E : Environment)
+  (J : JStackCtx cCnt defs)
+  (S : Store cCnt defs)
+  (K : List (Cont cCnt defs)) : CEK .Cont
 
 inductive liftValue : Value → Lang .Expr → Prop
 | True : liftValue .True .True
@@ -338,180 +340,191 @@ inductive ValueTyp : Value → Ty → (Store cCnt defs) → Prop
   ValueTyp (.Nat n) .nat S
 | Unit :
   ValueTyp .Unit .unit S
-| Cls (cls : Fin cCnt) (a : Addr) (S : Store cCnt defs) (vls : Fin (defs.fieldsCnt cls) → Value) :
+| Cls (cls : Fin cCnt)
+  (cls_tp : Nat)
+  (a : Addr) (S : Store cCnt defs) (vls : Fin (defs.fieldsCnt cls) → Value) :
   S.lookup a = .some (⟨cls, vls⟩ : Object cCnt defs) →
-  ∀ i, ValueTyp (vls i) (defs.fieldsTy cls i) S →
-  ValueTyp (.Addr a) (.cls cls) S
+  (∀ i, ValueTyp (vls i) (defs.fieldsTy cls i) S) →
+  cls_tp = cls.val →
+  ValueTyp (.Addr a) (.cls cls_tp) S
 
-inductive Eval : CEK cCnt defs → CEK cCnt defs → Prop
+inductive Eval : (m₁ : EvalMode) → (m₂ : EvalMode) → CEK cCnt defs m₁ → CEK cCnt defs m₂ → Prop
 -- # Expr
 | Val (v : Value) (e : Lang .Expr) :
   liftValue v e →
-  Eval
-    ⟨.sourceExpr e, E, J, S, K⟩
-    ⟨.value v, E, J, S, K⟩
+  Eval .Eval .Cont
+    (.Eval .Expr e E J S K)
+    (.Cont (.value v) E J S K)
 | Var (x : VarName) :
-  Eval
-    ⟨.sourceExpr (.Var x), E, J, S, K⟩
-    ⟨.value (E[x]!), E, J, S, K⟩
+  Eval .Eval .Cont
+    (.Eval .Expr (.Var x) E J S K)
+    (.Cont (.value (E[x]!)) E J S K)
 | Field (f : Nat) (p : Lang .Expr) :
-  Eval
-    ⟨.sourceExpr (.Field f p), E, J, S, K⟩
-    ⟨.sourceExpr p, E, J, S, (.fieldK f) :: K⟩
-| Return (e : Lang .Expr) (l : Nat) :
-  Eval
-    ⟨.sourceExpr (.Return l e), E, J, S, K⟩
-    ⟨.sourceExpr e, E, J, S, (.returnK l) :: K⟩
+  Eval .Eval .Eval
+    (.Eval .Expr (.Field f p) E J S K)
+    (.Eval .Expr p E J S ((.fieldK f) :: K))
 | VarDecl (type : Ty) (e : Lang .Expr) :
-  Eval
-    ⟨.sourceStmt (.Decl type e), E, J, S, K⟩
-    ⟨.sourceExpr e, E, J, S, (.declK type) :: K⟩
+  Eval .Eval .Eval
+    (.Eval .Stmt (.Decl type e) E J S K)
+    (.Eval .Expr e E J S ((.declK type) :: K))
 | Assign (x : VarName) (e : Lang .Expr) :
-  Eval
-    ⟨.sourceStmt (.Assign x e), E, J, S, K⟩
-    ⟨.sourceExpr e, E, J, S, (.assignK x) :: K⟩
+  Eval .Eval .Eval
+    (.Eval .Stmt (.Assign x e) E J S K)
+    (.Eval .Expr e E J S ((.assignK x) :: K))
 | Seq (s₁ s₂ : Lang .Stmt) :
-  Eval
-    ⟨.sourceStmt (.Seq s₁ s₂), E, J, S, K⟩
-    ⟨.sourceStmt s₁, E, J, S, (.seqK s₂) :: K⟩
+  Eval .Eval .Eval
+    (.Eval .Stmt (.Seq s₁ s₂) E J S K)
+    (.Eval .Stmt s₁ E J S ((.seqK s₂) :: K))
 | ExprStmt (e : Lang .Expr) :
-  Eval
-    ⟨.sourceStmt (.Do e), E, J, S, K⟩
-    ⟨.sourceExpr e, E, J, S, .exprStmtK :: K⟩
+  Eval .Eval .Eval
+    (.Eval .Stmt (.Do e) E J S K)
+    (.Eval .Expr e E J S (.exprStmtK :: K))
 | BinOp (e₁ e₂ : Lang .Expr) (op : BinOp) :
-  Eval
-    ⟨.sourceExpr (.BinOp e₁ e₂ op), E, J, S, K⟩
-    ⟨.sourceExpr e₁, E, J, S, (.binopLK op e₂) :: K⟩
+  Eval .Eval .Eval
+    (.Eval .Expr (.BinOp e₁ e₂ op) E J S K)
+    (.Eval .Expr e₁ E J S ((.binopLK op e₂) :: K))
 | UnOp (e : Lang .Expr) (op : UnOp) :
-  Eval
-    ⟨.sourceExpr (.UnOp e op), E, J, S, K⟩
-    ⟨.sourceExpr e, E, J, S, (.unopK op) :: K⟩
+  Eval .Eval .Eval
+    (.Eval .Expr (.UnOp e op) E J S K)
+    (.Eval .Expr e E J S ((.unopK op) :: K))
 | If (e : Lang .Expr) (s₁ s₂ : Lang .Expr) :
-  Eval
-    ⟨.sourceExpr (.If e s₁ s₂), E, J, S, K⟩
-    ⟨.sourceExpr e, E, J, S, (.ifCondK s₁ s₂) :: K⟩
+  Eval .Eval .Eval
+    (.Eval .Expr (.If e s₁ s₂) E J S K)
+    (.Eval .Expr e E J S ((.ifCondK s₁ s₂) :: K))
 | While (c : Lang .Expr) (body : Lang .Expr) :
-  Eval
-    ⟨.sourceExpr (.While c body), E, J, S, K⟩
-    ⟨.sourceExpr c, E, J, S, (.loopK c body E.length) :: K⟩
-| Break (K' : List (Cont cCnt defs)) (l : Nat):
-  Eval
-    ⟨.sourceExpr (.Break l), E, J, S, K⟩
-    ⟨.value .Unit, E.drop (E.length - J[l]!.1), J.drop (l + 1), S, J[l]!.2⟩
+  Eval .Eval .Eval
+    (.Eval .Expr (.While c body) E J S K)
+    (.Eval .Expr c E J S ((.loopK c body) :: K))
+| Break (l : Nat) :
+  Eval .Eval .Cont
+    (.Eval .Expr (.Break l) E J S K)
+    (.Cont (.value .Unit) E J S J[l]!)
 | Scope (s : Lang .Stmt) (e : Lang .Expr) :
-  Eval
-    ⟨.sourceExpr (.Scope s e), E, J, S, K⟩
-    ⟨.sourceStmt s, E, J, S, .scopeBodyK e E.length :: K⟩
+  Eval .Eval .Eval
+    (.Eval .Expr (.Scope s e) E J S K)
+    (.Eval .Stmt s E J S (.scopeBodyK e E.length J :: K))
+| Return (e : Lang .Expr):
+  Eval .Eval .Eval
+    (.Eval .Expr (.Return e l) E J S K)
+    (.Eval .Expr e E J S (.returnJumpK l :: K))
 | Call₀ (cls : Fin cCnt) (m : Fin (defs.methodsCnt cls))
   (args : Fin (defs.methods cls m).nArg → Lang .Expr) :
   (0 = (defs.methods cls m).nArg) →
-  Eval
-    ⟨.sourceExpr (.Call m cls args), E, J, S, K⟩
-    ⟨.sourceExpr (defs.methods cls m).body, [], ⟨E.length, K⟩ :: J, S,
-      (.callK E) :: K⟩
+  Eval .Eval .Eval
+    (.Eval .Expr (.Call m cls args) E J S K)
+    (.Eval .Expr (defs.methods cls m).body [] [.returnRestoreK E J :: K] S (.callRestoreK E J :: K))
 | Call (cls : Fin cCnt) (m : Fin (defs.methodsCnt cls))
   (args : Fin (defs.methods cls m).nArg → Lang .Expr) :
   (hn : 0 < (defs.methods cls m).nArg) →
-  Eval
-    ⟨.sourceExpr (.Call m cls args), E, J, S, K⟩
-    ⟨.sourceExpr (args ⟨0, hn⟩), E, J, S,
-      (.argK cls m ⟨0, hn⟩ (fun x => by grind [Fin]) (fun i => args ⟨i + 1, by grind⟩)) :: K⟩
+  Eval .Eval .Eval
+    (.Eval .Expr (.Call m cls args) E J S K)
+    (.Eval .Expr (args ⟨0, hn⟩) E J S
+      ((.argK cls m ⟨0, hn⟩ (fun x => by grind [Fin]) (fun i => args ⟨i + 1, by grind⟩)) :: K))
 | New₀ (cls : Fin cCnt) (a : Addr)
   (args : Fin (defs.fieldsCnt cls) → Lang .Expr) :
   (h0 : 0 = defs.fieldsCnt cls) →
   (ha : a ∉ S) →
-  Eval
-    ⟨.sourceExpr (.New cls args), E, J, S, K⟩
-    ⟨.value (.Addr a), E, J, S.insert a ⟨cls, fun _ => by grind [Fin]⟩, K⟩
+  Eval .Eval .Cont
+    (.Eval .Expr (.New cls args) E J S K)
+    (.Cont (.value (.Addr a)) E J (S.insert a ⟨cls, fun _ => by grind [Fin]⟩) K)
 | New (cls : Fin cCnt)
   (args : Fin (defs.fieldsCnt cls) → Lang .Expr) :
   (hn : 0 < defs.fieldsCnt cls) →
-  Eval
-    ⟨.sourceExpr (.Call m cls args), E, J, S, K⟩
-    ⟨.sourceExpr (args ⟨0, hn⟩), E, J, S,
-      (.newK cls ⟨0, hn⟩ (fun x => by grind [Fin]) (fun i => args ⟨i + 1, by grind⟩)) :: K⟩
+  Eval .Eval .Eval
+    (.Eval .Expr (.New cls args) E J S K)
+    (.Eval .Expr (args ⟨0, hn⟩) E J S
+      ((.newK cls ⟨0, hn⟩ (fun x => by grind [Fin]) (fun i => args ⟨i + 1, by grind⟩)) :: K))
 -- # Cont
 | FieldDone (a : Addr) (cls : Fin cCnt) (k : Fin (defs.fieldsCnt cls))
   (values : Fin (defs.fieldsCnt cls) → Value) :
   S.lookup a = some ⟨cls, values⟩ →
-  Eval
-    ⟨.value (.Addr a), E, J, S, (.fieldK k) :: K⟩
-    ⟨.value (values k), E, J, S, K⟩
-| IfTrue (s₁ s₂ : Lang .Expr) :
-  Eval
-    ⟨.value .True, E, J, S, .ifCondK s₁ s₂ :: K⟩
-    ⟨.sourceExpr s₁, E, J, S, K⟩
-| IfFalse (s₁ s₂ : Lang .Expr) :
-  Eval
-    ⟨.value .False, E, J, S, .ifCondK s₁ s₂ :: K⟩
-    ⟨.sourceExpr s₂, E, J, S, K⟩
-| ReturnDone (v : Value) (l : Nat) :
-  Eval
-    ⟨.value v, E, J, S, (.returnK l) :: K⟩
-    ⟨.value v, E.drop (E.length - J[l]!.1), J.drop (l + 1), S, J[l]!.2⟩
+  Eval .Cont .Cont
+    (.Cont (.value (.Addr a)) E J S ((.fieldK k) :: K))
+    (.Cont (.value (values k)) E J S K)
 | VarDeclDone (type : Ty) (v : Value) :
-  Eval
-    ⟨.value v, E, J, S, .declK type :: K⟩
-    ⟨.skip, v :: E, J, S, K⟩
+  Eval .Cont .Cont
+    (.Cont (.value v) E J S (.declK type :: K))
+    (.Cont .skip (v :: E) J S K)
 | AssignDone (x : VarName) (v : Value) :
-  Eval
-    ⟨.value v, E, J, S, .assignK x :: K⟩
-    ⟨.skip, E.set x v, J, S, K⟩
+  Eval .Cont .Cont
+    (.Cont (.value v) E J S (.assignK x :: K))
+    (.Cont .skip (E.set x v) J S K)
 | SeqDone (s₂ : Lang .Stmt) :
-  Eval
-    ⟨.skip, E, J, S, .seqK s₂ :: K⟩
-    ⟨.sourceStmt s₂, E, J, S, K⟩
+  Eval .Cont .Eval
+    (.Cont .skip E J S (.seqK s₂ :: K))
+    (.Eval .Stmt s₂ E J S K)
 | ExprStmtDone (v : Value) :
-  Eval
-    ⟨.value v, E, J, S, .exprStmtK :: K⟩
-    ⟨.skip, E, J, S, K⟩
+  Eval .Cont .Cont
+    (.Cont (.value v) E J S (.exprStmtK :: K))
+    (.Cont .skip E J S K)
 | BinOpL (op : BinOp) (v₁ : Value) (e₂ : Lang .Expr) :
-  Eval
-    ⟨.value v₁, E, J, S, .binopLK op e₂ :: K⟩
-    ⟨.sourceExpr e₂, E, J, S, .binopRK op v₁ :: K⟩
+  Eval .Cont .Eval
+    (.Cont (.value v₁) E J S (.binopLK op e₂ :: K))
+    (.Eval .Expr e₂ E J S (.binopRK op v₁ :: K))
 | BinOpR (op : BinOp) (v₁ v₂ result : Value) :
   op.step v₁ v₂ result →
-  Eval
-    ⟨.value v₂, E, J, S, .binopRK op v₁ :: K⟩
-    ⟨.value result, E, J, S, K⟩
+  Eval .Cont .Cont
+    (.Cont (.value v₂) E J S (.binopRK op v₁ :: K))
+    (.Cont (.value result) E J S K)
 | UnOpDone (op : UnOp) (v result : Value) :
   op.step v result →
-  Eval
-    ⟨.value v, E, J, S, .unopK op :: K⟩
-    ⟨.value result, E, J, S, K⟩
-| LoopTrue (body : Lang .Expr) (c : Lang .Expr) (n : Nat) :
-  Eval
-    ⟨.value .True, E, J, S, .loopK c body n :: K⟩
-    ⟨.sourceExpr body, E, ⟨n, K⟩ :: J, S, .loopContK c body n :: K⟩
+  Eval .Cont .Cont
+    (.Cont (.value v) E J S (.unopK op :: K))
+    (.Cont (.value result) E J S K)
+| IfTrue (s₁ s₂ : Lang .Expr) :
+  Eval .Cont .Eval
+    (.Cont (.value .True) E J S (.ifCondK s₁ s₂ :: K))
+    (.Eval .Expr s₁ E J S K)
+| IfFalse (s₁ s₂ : Lang .Expr) :
+  Eval .Cont .Eval
+    (.Cont (.value .False) E J S (.ifCondK s₁ s₂ :: K))
+    (.Eval .Expr s₂ E J S K)
+| LoopTrue (body : Lang .Expr) (c : Lang .Expr) :
+  Eval .Cont .Eval
+    (.Cont (.value .True) E J S (.loopK c body :: K))
+    (.Eval .Expr body E ((.breakRestoreK E.length J :: K) :: J) S (.loopContK c body E.length J :: K))
 | LoopFalse (body : Lang .Expr) (c : Lang .Expr) (n : Nat) :
-  Eval
-    ⟨.value .False, E, J, S, .loopK c body n :: K⟩
-    ⟨.value .Unit, E.drop (E.length - n), J, S, K⟩
-| LoopCont (body : Lang .Expr) (c : Lang .Expr) (n : Nat) (K' : List (Cont cCnt defs)) :
-  Eval
-    ⟨.value .Unit, E, ⟨n, K⟩ :: J, S, .loopContK c body n :: K'⟩
-    ⟨.sourceExpr c, E, J, S, .loopK c body n :: K⟩
+  Eval .Cont .Cont
+    (.Cont (.value .False) E J S (.loopK c body :: K))
+    (.Cont (.value .Unit) E J S K)
+| LoopCont (body : Lang .Expr) (c : Lang .Expr) (n : Nat) :
+  Eval .Cont .Eval
+    (.Cont (.value .Unit) E J S (.loopContK c body n J₀ :: K))
+    (.Eval .Expr c (E.drop (E.length - n)) J₀ S (.loopK c body :: K))
+| BreakRestore :
+  Eval .Cont .Cont
+    (.Cont (.value .Unit) E J S (.breakRestoreK n J₀ :: K))
+    (.Cont (.value .Unit) (E.drop (E.length - n)) J₀ S K)
 | ScopeBody (body : Lang .Expr) (n : Nat) :
-  Eval
-    ⟨.skip, E, J, S, .scopeBodyK body n :: K⟩
-    ⟨.sourceExpr body, E, J, S, .scopeExitK n :: K⟩
-| ScopeExit (body : Lang .Expr) (n : Nat) (v : Value) :
-  Eval
-    ⟨.value v, E, J, S, .scopeExitK n :: K⟩
-    ⟨.value v, E.drop (E.length - n), J, S, K⟩
-| ArgNext (body : Lang .Expr)
-  (v : Value) (e : Lang .Expr)
+  Eval .Cont .Eval
+    (.Cont .skip E J S (.scopeBodyK body n J₀ :: K))
+    (.Eval .Expr body E J S (.scopeExitK n J₀ :: K))
+| ScopeExit (n : Nat) (v : Value) :
+  Eval .Cont .Cont
+    (.Cont (.value v) E J S (.scopeExitK n J₀ :: K))
+    (.Cont (.value v) (E.drop (E.length - n)) J₀ S K)
+| ReturnJump (v : Value) (l : Nat) :
+  J[l]! = K' →
+  Eval .Cont .Cont
+    (.Cont (.value v) E J S (.returnJumpK l :: K))
+    (.Cont (.value v) E J S K')
+| ReturnRestore (v : Value) :
+  Eval .Cont .Cont
+    (.Cont (.value v) E J S (.returnRestoreK E₀ J₀ :: K))
+    (.Cont (.value v) E₀ J₀ S K)
+| ArgNext
+  (v : Value)
   (cls : Fin cCnt) (m : Fin (defs.methodsCnt cls))
   (sep : Fin (defs.methods cls m).nArg)
   (vals : Fin sep → Value)
   (exprs : Fin ((defs.methods cls m).nArg - sep - 1) → Lang .Expr)
   (hn : sep + 1 < (defs.methods cls m).nArg) :
-  Eval
-    ⟨.value v, E, J, S, .argK cls m sep vals exprs :: K⟩
-    ⟨.sourceExpr e, E, J, S,
-      .argK cls m ⟨sep + 1, hn⟩
-      (fun i => if hs : i.val = sep.val then v else vals ⟨i, by grind⟩)
-      (fun i => exprs ⟨i + 1, by grind⟩) :: K⟩
+  Eval .Cont .Eval
+    (.Cont (.value v) E J S (.argK cls m sep vals exprs :: K))
+    (.Eval .Expr (exprs ⟨0, by omega⟩) E J S
+      (.argK cls m ⟨sep + 1, hn⟩
+        (fun i => if hs : i.val = sep.val then v else vals ⟨i, by grind⟩)
+        (fun i => exprs ⟨i + 1, by grind⟩) :: K))
 | ArgDone
   (v : Value)
   (cls : Fin cCnt) (m : Fin (defs.methodsCnt cls))
@@ -519,24 +532,28 @@ inductive Eval : CEK cCnt defs → CEK cCnt defs → Prop
   (vals : Fin sep → Value)
   (exprs : Fin ((defs.methods cls m).nArg - sep - 1) → Lang .Expr)
   (hn : sep + 1 = (defs.methods cls m).nArg) :
-  Eval
-    ⟨.value v, E, J, S, .argK cls m sep vals exprs :: K⟩
-    ⟨.sourceExpr (defs.methods cls m).body,
-      List.ofFn (fun i => if hs : i = sep then v else vals ⟨i, by grind⟩),
-      J, S, .callK E :: K⟩
+  Eval .Cont .Eval
+    (.Cont (.value v) E J S (.argK cls m sep vals exprs :: K))
+    (.Eval .Expr (defs.methods cls m).body
+      (List.ofFn (fun i => if hs : i = sep then v else vals ⟨i, by grind⟩))
+      ([.returnRestoreK E J :: K]) S (.callRestoreK E J :: K))
+| CallRestore (v : Value) :
+  Eval .Cont .Cont
+    (.Cont (.value v) E J S (.callRestoreK E₀ J₀ :: K))
+    (.Cont (.value v) E₀ J₀ S K)
 | NewNext
-  (v : Value) (e : Lang .Expr)
+  (v : Value)
   (cls : Fin cCnt)
   (sep : Fin (defs.fieldsCnt cls))
   (vals : Fin sep → Value)
   (exprs : Fin (defs.fieldsCnt cls - sep - 1) → Lang .Expr)
   (hn : sep + 1 < defs.fieldsCnt cls) :
-  Eval
-    ⟨.value v, E, J, S, .newK cls sep vals exprs :: K⟩
-    ⟨.sourceExpr e, E, J, S,
-      .newK cls ⟨sep + 1, hn⟩
-      (fun i => if hs : i.val = sep.val then v else vals ⟨i, by grind⟩)
-      (fun i => exprs ⟨i + 1, by grind⟩) :: K⟩
+  Eval .Cont .Eval
+    (.Cont (.value v) E J S (.newK cls sep vals exprs :: K))
+    (.Eval .Expr (exprs ⟨0, by omega⟩) E J S
+      (.newK cls ⟨sep + 1, hn⟩
+        (fun i => if hs : i.val = sep.val then v else vals ⟨i, by grind⟩)
+        (fun i => exprs ⟨i + 1, by grind⟩) :: K))
 | NewDone
   (v : Value)
   (cls : Fin cCnt)
@@ -544,26 +561,30 @@ inductive Eval : CEK cCnt defs → CEK cCnt defs → Prop
   (vals : Fin sep → Value)
   (exprs : Fin (defs.fieldsCnt cls - sep - 1) → Lang .Expr)
   (hn : sep + 1 = defs.fieldsCnt cls) (a : Addr) (ha : a ∉ S) :
-  Eval
-    ⟨.value v, E, J, S, .newK cls sep vals exprs :: K⟩
-    ⟨.value (.Addr a), E, J,
-      S.insert a ⟨cls, (fun i => if hs : i.val = sep.val then v else vals ⟨i, by grind⟩)⟩,
-      .callK E :: K⟩
+  Eval .Cont .Cont
+    (.Cont (.value v) E J S (.newK cls sep vals exprs :: K))
+    (.Cont (.value (.Addr a)) E J
+      (S.insert a ⟨cls, (fun i => if hs : i.val = sep.val then v else vals ⟨i, by grind⟩)⟩)
+      K)
 
 
 
-def initState (s : Lang .Stmt) : CEK cCnt defs := ⟨.sourceStmt s, [], [], ∅, []⟩
+def initState (cls : Fin cCnt) (m : Fin (defs.methodsCnt cls)) : CEK cCnt defs .Eval :=
+  .Eval .Expr (defs.methods cls m).body [] [] ∅ []
 
-def terminalState (E : Environment) (J : JStackCtx cCnt defs) (S : Store cCnt defs) :
-  CEK cCnt defs := ⟨.skip, E, J, S, []⟩
+def terminalState :
+  CEK cCnt defs m → Prop
+| .Cont (.value _) _ _ S [] => True
+| _ => False
 
 inductive ContTypeRes : Tag → Type
 | Expr (type : Ty) : ContTypeRes .Expr
 | Stmt : ContTypeRes .Stmt
 
-def ctx_limit (n : Nat) : JCtx → Prop
+def ctx_limit (n : Nat) : JCtx cCnt defs → Prop
 | [] => True
-| x :: _ => x ≤ n
+| .Loop x :: _ => x ≤ n
+| _ => True
 
 inductive Coh : Environment → (Store cCnt defs) → Ctx → Prop
 | CohEmp :
@@ -575,194 +596,303 @@ inductive Coh : Environment → (Store cCnt defs) → Ctx → Prop
 
 -- # Expression Continuations
 inductive ContType : (tg : Tag) →
-  (cCur : Fin cCnt) → (Fin (defs.methodsCnt cCur)) →
-  JCtx → Ctx → List (Cont cCnt defs) → ContTypeRes tg → Prop
-| IfCondK
-  (cCur : Fin cCnt) (mCur : Fin (defs.methodsCnt cCur))
-  (s₁ : Lang .Expr) (s₂ : Lang .Expr) (Γ₁ : Ctx) (type : Ty) :
-  Typ cCnt defs .Expr cCur mCur Δ₁ Γ₁ s₁ (.Expr type) →
-  Typ cCnt defs .Expr cCur mCur Δ₁ Γ₁ s₂ (.Expr type) →
-  ContType .Expr cCur mCur Δ₁ Γ₁ K (.Expr type) →
-  ContType .Expr cCur mCur Δ₁ Γ₁ (.ifCondK s₁ s₂ :: K) (.Expr .bool)
+  JCtx cCnt defs → Ctx → Store cCnt defs → List (Cont cCnt defs) → ContTypeRes tg → Prop
+| EmptyValueK (ty : Ty) :
+  ContType .Expr Δ Γ S [] (.Expr ty)
+| FieldK
+  (cls : Fin cCnt) (ty : Ty) (f : Nat) (hf : f < defs.fieldsCnt cls) :
+  defs.fieldsTy cls ⟨f, hf⟩ = ty →
+  ContType .Expr Δ₁ Γ₁ S K (.Expr ty) →
+  ContType .Expr Δ₁ Γ₁ S (.fieldK f :: K) (.Expr (.cls cls))
 | DeclK
-  (cCur : Fin cCnt) (mCur : Fin (defs.methodsCnt cCur))
   (type : Ty) (Γ₁ : Ctx) :
-  ContType .Stmt cCur mCur Δ₁ (type :: Γ₁) K .Stmt →
-  ContType .Expr cCur mCur Δ₁ Γ₁ (.declK type :: K) (.Expr type)
+  ContType .Stmt Δ₁ (type :: Γ₁) S K .Stmt →
+  ContType .Expr Δ₁ Γ₁ S (.declK type :: K) (.Expr type)
 | AssignK
-  (cCur : Fin cCnt) (mCur : Fin (defs.methodsCnt cCur))
   (x : VarName) (type : Ty) (Γ₁ : Ctx) :
   (Γ₁(x) = type) →
-  ContType .Stmt cCur mCur Δ₁ Γ₁ K .Stmt →
-  ContType .Expr cCur mCur Δ₁ Γ₁ (.assignK x :: K) (.Expr type)
+  ContType .Stmt Δ₁ Γ₁ S K .Stmt →
+  ContType .Expr Δ₁ Γ₁ S (.assignK x :: K) (.Expr type)
+| ExprStmtK
+  (Γ₁ : Ctx) (type : Ty) :
+  ContType .Stmt Δ₁ Γ₁ S K .Stmt →
+  ContType .Expr Δ₁ Γ₁ S (.exprStmtK :: K) (.Expr type)
 | BinOpLK
-  (cCur : Fin cCnt) (mCur : Fin (defs.methodsCnt cCur))
   (Γ₁ : Ctx) (op : BinOp) (e₂ : Lang .Expr) :
-  Typ cCnt defs .Expr cCur mCur Δ₁ Γ₁ e₂ (.Expr op.args.2) →
-  ContType .Expr cCur mCur Δ₁ Γ₁ K (.Expr op.args.out) →
-  ContType .Expr cCur mCur Δ₁ Γ₁ (.binopLK op e₂ :: K) (.Expr op.args.1)
+  Typ cCnt defs .Expr Δ₁ Γ₁ e₂ (.Expr op.args.2) →
+  ContType .Expr Δ₁ Γ₁ S K (.Expr op.args.out) →
+  ContType .Expr Δ₁ Γ₁ S (.binopLK op e₂ :: K) (.Expr op.args.1)
 | BinOpRK
-  (cCur : Fin cCnt) (mCur : Fin (defs.methodsCnt cCur))
   (Γ₁ : Ctx) (op : BinOp) (v₁ : Value) :
-  value_type v₁ op.args.1 →
-  ContType .Expr cCur mCur Δ₁ Γ₁ K (.Expr op.args.out) →
-  ContType .Expr cCur mCur Δ₁ Γ₁ (.binopRK op v₁ :: K) (.Expr op.args.2)
+  simpleType v₁ op.args.1 →
+  ContType .Expr Δ₁ Γ₁ S K (.Expr op.args.out) →
+  ContType .Expr Δ₁ Γ₁ S (.binopRK op v₁ :: K) (.Expr op.args.2)
 | UnOpK
-  (cCur : Fin cCnt) (mCur : Fin (defs.methodsCnt cCur))
   (Γ₁ : Ctx) (op : UnOp) :
-  ContType .Expr cCur mCur Δ₁ Γ₁ K (.Expr op.args.out) →
-  ContType .Expr cCur mCur Δ₁ Γ₁ (.unopK op :: K) (.Expr op.args.1)
-| ReturnK
-  (cCur : Fin cCnt) (mCur : Fin (defs.methodsCnt cCur)) :
-  ContType .Expr cCur mCur Δ₁ Γ₁ (.returnK l :: K) (.Expr (defs.methods cCur mCur).ret)
-| FieldK
-  (cCur : Fin cCnt) (mCur : Fin (defs.methodsCnt cCur))
-  (cls : Fin cCnt) (ty : Ty) (f : Fin (defs.fieldsCnt cls)) :
-  defs.fieldsTy cls f = ty →
-  ContType .Expr cCur mCur Δ₁ Γ₁ K (.Expr ty) →
-  ContType .Expr cCur mCur Δ₁ Γ₁ (.fieldK f :: K) (.Expr (.cls cls))
+  ContType .Expr Δ₁ Γ₁ S K (.Expr op.args.out) →
+  ContType .Expr Δ₁ Γ₁ S (.unopK op :: K) (.Expr op.args.1)
+| IfCondK
+  (s₁ : Lang .Expr) (s₂ : Lang .Expr) (Γ₁ : Ctx) (type : Ty) :
+  Typ cCnt defs .Expr Δ₁ Γ₁ s₁ (.Expr type) →
+  Typ cCnt defs .Expr Δ₁ Γ₁ s₂ (.Expr type) →
+  ContType .Expr Δ₁ Γ₁ S K (.Expr type) →
+  ContType .Expr Δ₁ Γ₁ S (.ifCondK s₁ s₂ :: K) (.Expr .bool)
+| LoopK
+  (Γ₁ : Ctx) (e : Lang .Expr) (c : Lang .Expr) :
+  Typ cCnt defs .Expr Δ₁ Γ₁ c (.Expr .bool) →
+  Typ cCnt defs .Expr (.Loop Γ₁.length :: Δ₁) Γ₁ e (.Expr .unit) →
+  ContType .Expr Δ₁ Γ₁ S K (.Expr .unit) →
+  ContType .Expr Δ₁ Γ₁ S (.loopK c e :: K) (.Expr .bool)
+| LoopContK
+  (Γ₁ : Ctx) (e : Lang .Expr) (c : Lang .Expr)
+  (cnts : List (List (Cont cCnt defs))) :
+  --add coherence
+  n ≤ Γ₁.length →
+  Typ cCnt defs .Expr Δ₁ (Γ₁.drop (Γ₁.length - n)) c (.Expr .bool) →
+  Typ cCnt defs .Expr (.Loop n :: Δ₁) (Γ₁.drop (Γ₁.length - n)) e (.Expr .unit) →
+  Δ₁.length = J₀.length →
+  Δ₁.length = cnts.length →
+  (∀ l < J₀.length, ∀ n1,
+    (Δ₁[l]! = .Loop n1 →
+   ContType .Expr Δ₁ (Γ₁.drop (Γ₁.length - n)) S J₀[l]! (.Expr .unit))) →
+  (∀ l < J₀.length, ∀ n1,
+    (Δ₁[l]! = .Loop n1 → ∃ J₁, J₀[l]! = .breakRestoreK n1 J₁ :: cnts[l]!)) →
+  (∀ l < J₀.length, ∀ cls m,
+    (Δ₁[l]! = .Method cls m →
+    ContType .Expr Δ₁ Γ₁ S J₀[l]! (.Expr (defs.methods cls m).ret))) →
+  (∀ l < J₀.length, ∀ cls m,
+    (Δ₁[l]! = .Method cls m → ∃ E₀ J₁, J₀[l]! = .returnRestoreK E₀ J₁ :: cnts[l]!)) →
+  ContType .Expr Δ₁ (Γ₁.drop (Γ₁.length - n)) S K (.Expr .unit) →
+  ContType .Expr (.Loop Γ₁.length :: Δ₁) Γ₁ S (.loopContK c e n J₀ :: K) (.Expr .unit)
+| BreakRestoreK (Γ₁ : Ctx)
+  (cnts : List (List (Cont cCnt defs))) :
+  --add coherence
+  n ≤ Γ₁.length →
+  Δ₁.length = J₀.length →
+  Δ₁.length = cnts.length →
+  (∀ l < J₀.length, ∀ n1,
+    (Δ₁[l]! = .Loop n1 →
+   ContType .Expr Δ₁ (Γ₁.drop (Γ₁.length - n)) S J₀[l]! (.Expr .unit))) →
+  (∀ l < J₀.length, ∀ n1,
+    (Δ₁[l]! = .Loop n1 → ∃ J₁, J₀[l]! = .breakRestoreK n1 J₁ :: cnts[l]!)) →
+  (∀ l < J₀.length, ∀ cls m,
+    (Δ₁[l]! = .Method cls m →
+    ContType .Expr Δ₁ (Γ₁.drop (Γ₁.length - n)) S J₀[l]! (.Expr (defs.methods cls m).ret))) →
+  (∀ l < J₀.length, ∀ cls m,
+    (Δ₁[l]! = .Method cls m → ∃ E₀ J₁, J₀[l]! = .returnRestoreK E₀ J₁ :: cnts[l]!)) →
+  ContType .Expr Δ₁ (Γ₁.drop (Γ₁.length - n)) S K (.Expr .unit) →
+  ContType .Expr Δ Γ₁ S (.breakRestoreK n J₀ :: K) (.Expr .unit)
+| ScopeExitK
+  (Γ₁ : Ctx) (n : Nat) (type : Ty)
+  (cnts : List (List (Cont cCnt defs))) :
+  --add coherence
+  n ≤ Γ₁.length →
+  Δ₂.length = J₀.length →
+  Δ₂.length = cnts.length →
+  (∀ l < J₀.length, ∀ n1,
+    (Δ₂[l]! = .Loop n1 →
+   ContType .Expr Δ₂ (Γ₁.drop (Γ₁.length - n)) S J₀[l]! (.Expr .unit))) →
+  (∀ l < J₀.length, ∀ n1,
+    (Δ₂[l]! = .Loop n1 → ∃ J₁, J₀[l]! = .breakRestoreK n1 J₁ :: cnts[l]!)) →
+  (∀ l < J₀.length, ∀ cls m,
+    (Δ₂[l]! = .Method cls m →
+    ContType .Expr Δ₂ Γ₁ S J₀[l]! (.Expr (defs.methods cls m).ret))) →
+  (∀ l < J₀.length, ∀ cls m,
+    (Δ₂[l]! = .Method cls m → ∃ E₀ J₁, J₀[l]! = .returnRestoreK E₀ J₁ :: cnts[l]!)) →
+  ContType .Expr Δ₂ (Γ₁.drop (Γ₁.length - n)) S K (.Expr type) →
+  ContType .Expr Δ₁ Γ₁ S (.scopeExitK n J₀ :: K) (.Expr type)
+| ReturnJumpK
+  (cls : Fin cCnt) (m : Fin (defs.methodsCnt cls))
+  (ret : Ty) (l : Nat) :
+  l < Δ₁.length →
+  Δ₁[l]! = .Method cls m →
+  -- is this one needed?
+  (l = 0 ∨ LoopJump cCnt defs Δ₁ (l - 1)) →
+  ret = (defs.methods cls m).ret →
+  ContType .Expr Δ₁ Γ₁ S (.returnJumpK l :: K) (.Expr ret)
+| ReturnRestoreK (ty : Ty) (J₀ : JStackCtx cCnt defs)
+  (cnts : List (List (Cont cCnt defs))) :
+  --add coherence
+  Coh cCnt defs E₀ S Γ₂ →
+  Δ₂.length = J₀.length →
+  Δ₂.length = cnts.length →
+  (∀ l < J₀.length, ∀ n1,
+    (Δ₂[l]! = .Loop n1 →
+   ContType .Expr Δ₂ Γ₂ S J₀[l]! (.Expr .unit))) →
+  (∀ l < J₀.length, ∀ n1,
+    (Δ₂[l]! = .Loop n1 → ∃ J₁, J₀[l]! = .breakRestoreK n1 J₁ :: cnts[l]!)) →
+  (∀ l < J₀.length, ∀ cls m,
+    (Δ₂[l]! = .Method cls m →
+    ContType .Expr Δ₂ Γ₂ S J₀[l]! (.Expr (defs.methods cls m).ret))) →
+  (∀ l < J₀.length, ∀ cls m,
+    (Δ₂[l]! = .Method cls m → ∃ E₀ J₁, J₀[l]! = .returnRestoreK E₀ J₁ :: cnts[l]!)) →
+  ContType .Expr Δ₂ Γ₂ S K (.Expr ty) →
+  ContType .Expr Δ₁ Γ₁ S (.returnRestoreK E₀ J₀ :: K) (.Expr ty)
+| CallRestoreK (ty : Ty)
+  (cnts : List (List (Cont cCnt defs))) :
+  --add coherence
+  Coh cCnt defs E₀ S Γ₂ →
+  Δ₂.length = J₀.length →
+  Δ₂.length = cnts.length →
+  (∀ l < J₀.length, ∀ n1,
+    (Δ₂[l]! = .Loop n1 →
+   ContType .Expr Δ₂ Γ₂ S J₀[l]! (.Expr .unit))) →
+  (∀ l < J₀.length, ∀ n1,
+    (Δ₂[l]! = .Loop n1 → ∃ J₁, J₀[l]! = .breakRestoreK n1 J₁ :: cnts[l]!)) →
+  (∀ l < J₀.length, ∀ cls m,
+    (Δ₂[l]! = .Method cls m →
+    ContType .Expr Δ₂ Γ₂ S J₀[l]! (.Expr (defs.methods cls m).ret))) →
+  (∀ l < J₀.length, ∀ cls m,
+    (Δ₂[l]! = .Method cls m → ∃ E₀ J₁, J₀[l]! = .returnRestoreK E₀ J₁ :: cnts[l]!)) →
+  ContType .Expr Δ₂ Γ₂ S K (.Expr ty) →
+  ContType .Expr Δ₁ Γ₁ S (.callRestoreK E₀ J₀ :: K) (.Expr ty)
 | ArgK
-  (cCur : Fin cCnt) (mCur : Fin (defs.methodsCnt cCur))
   (cls : Fin cCnt) (m : Fin (defs.methodsCnt cls))
   (sep : Fin (defs.methods cls m).nArg) (vals : Fin sep → Value)
   (exprs : Fin ((defs.methods cls m).nArg - sep - 1) → Lang .Expr)
   (retTy : Ty) (tyRes : Ty) :
   retTy = (defs.methods cls m).ret →
   tyRes = (defs.methods cls m).argTy sep →
-  /- do we even need this?
   (∀ i,
-    ValueTyp cCnt defs (vals i) ((defs.methods cls m).argTy ⟨i, by omega⟩) S) →-/
+    ValueTyp cCnt defs (vals i) ((defs.methods cls m).argTy ⟨i, by omega⟩) S) →
   (∀ i,
-    Typ cCnt defs .Expr cCur mCur Δ₁ Γ₁
+    Typ cCnt defs .Expr Δ₁ Γ₁
       (exprs i)
       (.Expr ((defs.methods cls m).argTy ⟨i + sep + 1, by omega⟩))) →
-  ContType .Expr cCur mCur Δ₁ Γ₁ K (.Expr retTy) →
-  ContType .Expr cCur mCur Δ₁ Γ₁ (.argK cls m sep vals exprs :: K) (.Expr tyRes)
+  ContType .Expr Δ₁ Γ₁ S K (.Expr retTy) →
+  ContType .Expr Δ₁ Γ₁ S (.argK cls m sep vals exprs :: K) (.Expr tyRes)
 | NewK
-  (cCur : Fin cCnt) (mCur : Fin (defs.methodsCnt cCur))
   (cls : Fin cCnt)
   (sep : Fin (defs.fieldsCnt cls)) (vals : Fin sep → Value)
   (exprs : Fin (defs.fieldsCnt cls - sep - 1) → Lang .Expr)
   (retTy : Ty) (tyRes : Ty) :
   retTy = .cls cls →
   tyRes = (defs.fieldsTy cls sep) →
-  /- do we even need this?
   (∀ i,
-    ValueTyp cCnt defs (vals i) (defs.fieldsTy cls ⟨i, by omega⟩) S) →-/
+    ValueTyp cCnt defs (vals i) (defs.fieldsTy cls ⟨i, by omega⟩) S) →
   (∀ i,
-    Typ cCnt defs .Expr cCur mCur Δ₁ Γ₁
+    Typ cCnt defs .Expr Δ₁ Γ₁
       (exprs i)
       (.Expr (defs.fieldsTy cls ⟨i + sep + 1, by omega⟩))) →
-  ContType .Expr cCur mCur Δ₁ Γ₁ K (.Expr retTy) →
-  ContType .Expr cCur mCur Δ₁ Γ₁ (.newK cls sep vals exprs :: K) (.Expr tyRes)
-| LoopK
-  (cCur : Fin cCnt) (mCur : Fin (defs.methodsCnt cCur))
-  (Γ₁ : Ctx) (e : Lang .Expr) (c : Lang .Expr) :
-  Typ cCnt defs .Expr cCur mCur Δ₁ Γ₁ c (.Expr .bool) →
-  Typ cCnt defs .Expr cCur mCur (Γ₁.length :: Δ₁) Γ₁ e (.Expr .unit) →
-  ContType .Expr cCur mCur Δ₁ Γ₁ K (.Expr .unit) →
-  ContType .Expr cCur mCur Δ₁ Γ₁ (.loopK c e Γ₁.length :: K) (.Expr .bool)
-| LoopContK
-  (cCur : Fin cCnt) (mCur : Fin (defs.methodsCnt cCur))
-  (Γ₁ : Ctx) (e : Lang .Expr) (c : Lang .Expr) :
-  Typ cCnt defs .Expr cCur mCur Δ₁ Γ₁ c (.Expr .bool) →
-  Typ cCnt defs .Expr cCur mCur (Γ₁.length :: Δ₁) Γ₁ e (.Expr .unit) →
-  ContType .Expr cCur mCur Δ₁ Γ₁ K (.Expr .unit) →
-  ContType .Expr cCur mCur (Γ₁.length :: Δ₁) Γ₁ (.loopContK c e Γ₁.length :: K) (.Expr .unit)
-| ScopeExitK
-  (cCur : Fin cCnt) (mCur : Fin (defs.methodsCnt cCur))
-  (Γ₁ : Ctx) (n : Nat) (type : Ty) :
-  ctx_limit n Δ₁ →
-  ContType .Expr cCur mCur Δ₁ (Γ₁.drop (Γ₁.length - n)) K (.Expr type) →
-  ContType .Expr cCur mCur Δ₁ Γ₁ (.scopeExitK n :: K) (.Expr type)
-| ExprStmtK
-  (cCur : Fin cCnt) (mCur : Fin (defs.methodsCnt cCur))
-  (Γ₁ : Ctx) (type : Ty) :
-  ContType .Stmt cCur mCur Δ₁ Γ₁ K .Stmt →
-  ContType .Expr cCur mCur Δ₁ Γ₁ (.exprStmtK :: K) (.Expr type)
+  ContType .Expr Δ₁ Γ₁ S K (.Expr retTy) →
+  ContType .Expr Δ₁ Γ₁ S (.newK cls sep vals exprs :: K) (.Expr tyRes)
 -- # Statement Continuations
-| HaltK
-  (cCur : Fin cCnt) (mCur : Fin (defs.methodsCnt cCur))
-  (Γ₁ : Ctx) :
-  ContType .Stmt cCur mCur Δ₁ Γ₁ [] .Stmt
 | SeqK
-  (cCur : Fin cCnt) (mCur : Fin (defs.methodsCnt cCur))
   (Γ₁ : Ctx) (Γ₂ : Ctx) (s : Lang .Stmt) :
-  Typ cCnt defs .Stmt cCur mCur Δ₁ Γ₁ s (.Stmt Γ₂) →
-  ContType .Stmt cCur mCur Δ₁ Γ₂ K .Stmt →
-  ContType .Stmt cCur mCur Δ₁ Γ₁ (.seqK s :: K) .Stmt
+  Typ cCnt defs .Stmt Δ₁ Γ₁ s (.Stmt Γ₂) →
+  ContType .Stmt Δ₁ Γ₂ S K .Stmt →
+  ContType .Stmt Δ₁ Γ₁ S (.seqK s :: K) .Stmt
 | ScopeBodyK
-  (cCur : Fin cCnt) (mCur : Fin (defs.methodsCnt cCur))
-  (Γ₁ : Ctx) (e : Lang .Expr) (type : Ty) (n : Nat) :
-  Typ cCnt defs .Expr cCur mCur Δ₁ Γ₁ e (.Expr type) →
-  ctx_limit n Δ₁ →
-  ContType .Expr cCur mCur Δ₁ (Γ₁.drop (Γ₁.length - n)) K (.Expr type) →
-  ContType .Stmt cCur mCur Δ₁ Γ₁ (.scopeBodyK e n :: K) .Stmt
-| CallK
-  (cCur : Fin cCnt) (mCur : Fin (defs.methodsCnt cCur))
-  (Δ' : JCtx) (Γ' : Ctx) (ty : Ty) :
-  -- add which type is returned?
-  Coh cCnt defs E S Γ' →
-  ContType .Expr cCur mCur Δ' Γ' K (.Expr ty) →
-  ContType .Stmt cCur mCur Δ₁ Γ₁ (.callK E :: K) .Stmt
-
-inductive JCoh : JStackCtx cCnt defs → Ctx → JCtx → Prop
-| JCohEmp :
-  JCoh [] Γ []
-| JCohLoop
-  (cCur : Fin cCnt) (mCur : Fin (defs.methodsCnt cCur))
-  (n : Nat) (Γ₁ : Ctx) (Δ₁ : JCtx) :
+  (Γ₁ : Ctx) (e : Lang .Expr) (type : Ty) (n : Nat)
+  (cnts : List (List (Cont cCnt defs))) :
+  --add coherence
+  Typ cCnt defs .Expr Δ₁ Γ₁ e (.Expr type) →
   n ≤ Γ₁.length →
-  JCoh J (Γ₁.drop (Γ₁.length - n)) Δ₁ →
-  ContType cCnt defs .Expr cCur mCur Δ₁ (Γ₁.drop (Γ₁.length - n)) K (.Expr .unit) →
-  JCoh (⟨n, K⟩ :: J) Γ₁ (n :: Δ₁)
+  Δ₁.length = J₀.length →
+  Δ₁.length = cnts.length →
+  (∀ l < J₀.length, ∀ n1,
+    (Δ₁[l]! = .Loop n1 →
+   ContType .Expr Δ₁ (Γ₁.drop (Γ₁.length - n)) S J₀[l]! (.Expr .unit))) →
+  (∀ l < J₀.length, ∀ n1,
+    (Δ₁[l]! = .Loop n1 → ∃ J₁, J₀[l]! = .breakRestoreK n1 J₁ :: cnts[l]!)) →
+  (∀ l < J₀.length, ∀ cls m,
+    (Δ₁[l]! = .Method cls m →
+    ContType .Expr Δ₁ Γ₁ S J₀[l]! (.Expr (defs.methods cls m).ret))) →
+  (∀ l < J₀.length, ∀ cls m,
+    (Δ₁[l]! = .Method cls m → ∃ E₀ J₁, J₀[l]! = .returnRestoreK E₀ J₁ :: cnts[l]!)) →
+  ContType .Expr Δ₁ (Γ₁.drop (Γ₁.length - n)) S K (.Expr type) →
+  ContType .Stmt Δ₁ Γ₁ S (.scopeBodyK e n J₀ :: K) .Stmt
 
 def S_ok (S : Store cCnt defs) : Prop :=
   ∀ obj ∈ S.entries, (ValueTyp cCnt defs (.Addr obj.1) (.cls obj.2.cls) S)
 
 def defs_ok : Prop :=
   ∀ cls m,
-    Typ cCnt defs .Expr cls m []
+    Typ cCnt defs .Expr [.Method cls m]
       (List.ofFn (defs.methods cls m).argTy)
       (defs.methods cls m).body
       (.Expr (defs.methods cls m).ret)
 
-inductive Wt : CEK cCnt defs → Prop
+inductive Wt : (m : EvalMode) → CEK cCnt defs m → Prop
 | WtExprE
-  (cCur : Fin cCnt) (mCur : Fin (defs.methodsCnt cCur))
-  (e : Lang .Expr) (type : Ty) :
+  (e : Lang .Expr) (type : Ty)
+  (cnts : List (List (Cont cCnt defs))) :
   Coh cCnt defs E S Γ →
-  JCoh cCnt defs J Γ Δ →
   S_ok cCnt defs S →
   defs_ok cCnt defs →
-  Typ cCnt defs .Expr cCur mCur Δ Γ e (.Expr type) →
-  ContType cCnt defs .Expr cCur mCur Δ Γ K (.Expr type) →
-  Wt ⟨.sourceExpr e, E, J, S, K⟩
+  Typ cCnt defs .Expr Δ Γ e (.Expr type) →
+  Δ.length = J.length →
+  Δ.length = cnts.length →
+  (∀ l < J.length, ∀ n1,
+    (Δ[l]! = .Loop n1 →
+   ContType cCnt defs .Expr Δ Γ S J[l]! (.Expr .unit))) →
+  (∀ l < J.length, ∀ n1,
+    (Δ[l]! = .Loop n1 → ∃ J₁, J[l]! = .breakRestoreK n1 J₁ :: cnts[l]!)) →
+  (∀ l < J.length, ∀ cls m,
+    (Δ[l]! = .Method cls m →
+    ContType cCnt defs .Expr Δ Γ S J[l]! (.Expr (defs.methods cls m).ret))) →
+  (∀ l < J.length, ∀ cls m,
+    (Δ[l]! = .Method cls m → ∃ E₀ J₁, J[l]! = .returnRestoreK E₀ J₁ :: cnts[l]!)) →
+  ContType cCnt defs .Expr Δ Γ S K (.Expr type) →
+  Wt .Eval (.Eval .Expr e E J S K)
 | WtExprS
-  (cCur : Fin cCnt) (mCur : Fin (defs.methodsCnt cCur))
-  (s : Lang .Stmt) :
+  (s : Lang .Stmt)
+  (cnts : List (List (Cont cCnt defs))) :
   Coh cCnt defs E S Γ →
-  JCoh cCnt defs J Γ Δ →
   S_ok cCnt defs S →
   defs_ok cCnt defs →
-  Typ cCnt defs .Stmt cCur mCur Δ Γ s (.Stmt Γ₁) →
-  ContType cCnt defs .Stmt cCur mCur Δ Γ₁ K .Stmt →
-  Wt ⟨.sourceStmt s, E, J, S, K⟩
+  Typ cCnt defs .Stmt Δ Γ s (.Stmt Γ₁) →
+  Δ.length = J.length →
+  Δ.length = cnts.length →
+  (∀ l < J.length, ∀ n1,
+    (Δ[l]! = .Loop n1 →
+   ContType cCnt defs .Expr Δ Γ S J[l]! (.Expr .unit))) →
+  (∀ l < J.length, ∀ n1,
+    (Δ[l]! = .Loop n1 → ∃ J₁, J[l]! = .breakRestoreK n1 J₁ :: cnts[l]!)) →
+  (∀ l < J.length, ∀ cls m,
+    (Δ[l]! = .Method cls m →
+    ContType cCnt defs .Expr Δ Γ S J[l]! (.Expr (defs.methods cls m).ret))) →
+  (∀ l < J.length, ∀ cls m,
+    (Δ[l]! = .Method cls m → ∃ E₀ J₁, J[l]! = .returnRestoreK E₀ J₁ :: cnts[l]!)) →
+  ContType cCnt defs .Stmt Δ Γ₁ S K .Stmt →
+  Wt .Eval (.Eval .Stmt s E J S K)
 | WtContV
-  (cCur : Fin cCnt) (mCur : Fin (defs.methodsCnt cCur))
-  (v : Value) (type : Ty) :
+  (v : Value) (type : Ty)
+  (cnts : List (List (Cont cCnt defs))) :
   Coh cCnt defs E S Γ →
-  JCoh cCnt defs J Γ Δ →
   S_ok cCnt defs S →
   defs_ok cCnt defs →
   ValueTyp cCnt defs v type S →
-  ContType cCnt defs .Expr cCur mCur Δ Γ K (.Expr type) →
-  Wt ⟨.value v, E, J, S, K⟩
+  Δ.length = J.length →
+    Δ.length = cnts.length →
+  (∀ l < J.length, ∀ n1,
+    (Δ[l]! = .Loop n1 →
+   ContType cCnt defs .Expr Δ Γ S J[l]! (.Expr .unit))) →
+  (∀ l < J.length, ∀ n1,
+    (Δ[l]! = .Loop n1 → ∃ J₁, J[l]! = .breakRestoreK n1 J₁ :: cnts[l]!)) →
+  (∀ l < J.length, ∀ cls m,
+    (Δ[l]! = .Method cls m →
+    ContType cCnt defs .Expr Δ Γ S J[l]! (.Expr (defs.methods cls m).ret))) →
+  (∀ l < J.length, ∀ cls m,
+    (Δ[l]! = .Method cls m → ∃ E₀ J₁, J[l]! = .returnRestoreK E₀ J₁ :: cnts[l]!)) →
+  ContType cCnt defs .Expr Δ Γ S K (.Expr type) →
+  Wt .Cont (.Cont (.value v) E J S K)
 | WtContS
-  (cCur : Fin cCnt) (mCur : Fin (defs.methodsCnt cCur)) :
+  (cnts : List (List (Cont cCnt defs))) :
   Coh cCnt defs E S Γ →
-  JCoh cCnt defs J Γ Δ →
   S_ok cCnt defs S →
   defs_ok cCnt defs →
-  ContType cCnt defs .Stmt cCur mCur Δ Γ K .Stmt →
-  Wt ⟨.skip, E, J, S, K⟩
+  Δ.length = J.length →
+    Δ.length = cnts.length →
+  (∀ l < J.length, ∀ n1,
+    (Δ[l]! = .Loop n1 →
+   ContType cCnt defs .Expr Δ Γ S J[l]! (.Expr .unit))) →
+  (∀ l < J.length, ∀ n1,
+    (Δ[l]! = .Loop n1 → ∃ J₁, J[l]! = .breakRestoreK n1 J₁ :: cnts[l]!)) →
+  (∀ l < J.length, ∀ cls m,
+    (Δ[l]! = .Method cls m →
+    ContType cCnt defs .Expr Δ Γ S J[l]! (.Expr (defs.methods cls m).ret))) →
+  (∀ l < J.length, ∀ cls m,
+    (Δ[l]! = .Method cls m → ∃ E₀ J₁, J[l]! = .returnRestoreK E₀ J₁ :: cnts[l]!)) →
+  ContType cCnt defs .Stmt Δ Γ S K .Stmt →
+  Wt .Cont (.Cont .skip E J S K)
