lean-formalisation/LeanFormalisation/LClass/LClassExamples.lean
@@ -1,0 +1,5 @@
+/-
+How the examples are different from Kotlin? For example, no 'this' pointer.
+
+Missing key features: lambdas and inheritance.
+-/
