lean-formalisation/LeanFormalisation/LClass/Theorems/TypeProperties.lean
@@ -5,23 +5,10 @@ import LeanFormalisation.LClass.Theorems.Helpers
 
 variable (cCnt : Nat) (defs : Defs cCnt)
 
-theorem lang_det
-  (cCur : Fin cCnt) (mCur : Fin (defs.methodsCnt cCur))
-  (Γ₁ : Ctx) (tg : Tag) (Γ₂ Γ₃ : TypR tg) (s : Lang tg) (S : Store cCnt defs) :
-  Typ cCnt defs tg cCur mCur Δ₁ Γ₁ s Γ₂ →
-  Typ cCnt defs tg cCur mCur Δ₁ Γ₁ s Γ₃ → Γ₂ = Γ₃ := by
-    intro h1 h2
-    unhygienic induction h1 <;> try grind
-    all_goals try
-    { cases h2
-      grind }
-    stop sorry
-
 theorem typ_permutation
-  (cCur : Fin cCnt) (mCur : Fin (defs.methodsCnt cCur))
   (Γ₁ Γ₂ : Ctx) (tg : Tag) (Γ₃ : TypR tg) (e : Lang tg) :
   (∀ tp x, (Γ₁(x) = tp) ↔ Γ₂(x) = tp) →
-  Typ cCnt defs tg cCur mCur Δ₁ Γ₁ e Γ₃ → Typ cCnt defs tg cCur mCur Δ₁ Γ₂ e Γ₃ := by
+  Typ cCnt defs tg Δ₁ Γ₁ e Γ₃ → Typ cCnt defs tg Δ₁ Γ₂ e Γ₃ := by
     intro hg
     have leq : Γ₁.length = Γ₂.length := by
       by_cases h1: Γ₂.length < Γ₁.length
@@ -47,9 +34,8 @@ theorem typ_permutation
 
 
 lemma stmt_mono
-  (cCur : Fin cCnt) (mCur : Fin (defs.methodsCnt cCur))
   (Γ₁ : Ctx) (tg : Tag) (Γ₂ : TypR tg) (s : Lang tg) :
-  Typ cCnt defs tg cCur mCur Δ₁ Γ₁ s Γ₂ → ∃ Γ₃ : TypR tg, Γ₃.extR Γ₁ = Γ₂ := by
+  Typ cCnt defs tg Δ₁ Γ₁ s Γ₂ → ∃ Γ₃ : TypR tg, Γ₃.extR Γ₁ = Γ₂ := by
     intro hs
     unhygienic induction hs <;> try grind
     all_goals try
@@ -80,24 +66,73 @@ lemma stmt_mono
 
 
 lemma stmt_decl
-  (cCur : Fin cCnt) (mCur : Fin (defs.methodsCnt cCur))
   (type : Ty) :
-  Typ cCnt defs .Stmt cCur mCur Δ₁ Γ₁ (.Decl type e) (.Stmt Γ₂) → Γ₂ = type :: Γ₁ := by
+  Typ cCnt defs .Stmt Δ₁ Γ₁ (.Decl type e) (.Stmt Γ₂) → Γ₂ = type :: Γ₁ := by
   intro h
   cases h
   rfl
 
+lemma loop_jump_ext (Δ : JCtx cCnt defs) :
+  LoopJump cCnt defs Δ l ↔
+  (l < Δ.length ∧ ∀ i ≤ l, ∃ res, Δ[i]! = .Loop res):= by
+    constructor
+    { intro hl
+      induction hl
+      { simp }
+      constructor
+      { grind }
+      intro i hi
+      by_cases h0 : i = 0
+      { rw [h0]
+        simp }
+      rename_i a_ih
+      rcases a_ih.2 (i - 1) (by grind)
+      grind }
+    intro hall
+    induction l generalizing Δ
+    { cases Δ
+      { grind }
+      have := hall.2 0 (by simp)
+      grind [LoopJump] }
+    cases Δ
+    { grind }
+    rcases hall.2 0 (by simp) with ⟨res, hres⟩
+    simp at hres
+    simp only [hres]
+    apply LoopJump.Loop
+    simp only [Nat.add_one_sub_one]
+    rename_i a_ih _ _
+    apply a_ih
+    constructor
+    { grind }
+    intro i hi
+    rcases hall.2 (i + 1) (by omega)
+    grind
+
 theorem lang_extension
-  (cCur : Fin cCnt) (mCur : Fin (defs.methodsCnt cCur))
   (tg : Tag) (e : Lang tg) (res : TypR tg)
   (Γ₁ Γ₂ : Ctx) :
-    Typ cCnt defs tg cCur mCur Δ₁ Γ₁ e res →
-    Typ cCnt defs tg cCur mCur (Δ₁.map (fun x => x + Γ₂.length)) (Γ₁ ++ Γ₂) (e)
+    Typ cCnt defs tg Δ₁ Γ₁ e res →
+    Typ cCnt defs tg (Δ₁.map
+        (fun x => match x with
+          | .Loop n => .Loop (n + Γ₂.length)
+          | val => val))
+      (Γ₁ ++ Γ₂) e
       (res.extR Γ₂) := by
     intro h
-    unhygienic induction h generalizing Γ₂ <;>try solve_by_elim
+    unhygienic induction h generalizing Γ₂ <;> try solve_by_elim
     { rw [TypR.extR]
       apply Typ.VarAccess
+      grind }
+    { apply Typ.FieldAccess <;> solve_by_elim }
+    { apply Typ.Call <;> solve_by_elim }
+    { apply Typ.Return <;> try solve_by_elim
+      { grind }
+      { grind }
+      rcases a_1
+      { grind }
+      right
+      rw [loop_jump_ext] at *
       grind }
     { apply Typ.WhileExpr
       { solve_by_elim }
@@ -107,30 +142,68 @@ theorem lang_extension
         simp only [List.map_cons, List.length_append,
           TypR.extR] at h ⊢
         exact h } }
-    { exact Typ.BreakExpr cCur_1 mCur_1 .unit _
-        (by rw [List.length_map]; exact a) }
+    { apply Typ.BreakExpr
+      induction a <;> solve_by_elim }
     { solve_by_elim [Typ.ScopeExpr] }
     { rw [TypR.extR]
-      apply Typ.VarAssign _ _ _ _ _ (a_ih Γ₂)
+      apply Typ.VarAssign _ _ _ (a_ih Γ₂)
       grind }
     solve_by_elim [Typ.Seq]
 
 theorem typ_ext
-  (cCur : Fin cCnt) (mCur : Fin (defs.methodsCnt cCur))
   (e : Lang .Expr) (type : Ty) (Γ₁ Γ₂ : Ctx) :
-    Typ cCnt defs .Expr cCur mCur Δ₁ Γ₁ e (.Expr type) →
-    Typ cCnt defs .Expr cCur mCur (Δ₁.map (fun x => x + Γ₂.length)) (Γ₁ ++ Γ₂) e
+    Typ cCnt defs .Expr Δ₁ Γ₁ e (.Expr type) →
+    Typ cCnt defs .Expr (Δ₁.map
+        (fun x => match x with
+          | .Loop n => .Loop (n + Γ₂.length)
+          | val => val)) (Γ₁ ++ Γ₂) e
       (.Expr type) := by
     intro h
-    have lm := lang_extension cCnt defs _ _ _ _ _ _ Γ₂ h
+    have lm := lang_extension cCnt defs _ _ _ _ Γ₂ h
     rw [TypR.extR] at lm
     apply lm
 
 
 lemma lift_value_type
-  (cCur : Fin cCnt) (mCur : Fin (defs.methodsCnt cCur))
   (v : Value) (type : Ty) :
-  Typ cCnt defs .Expr cCur mCur Γ Δ e (.Expr type) →
+  Typ cCnt defs .Expr Γ Δ e (.Expr type) →
   liftValue v e → ValueTyp cCnt defs v type S := by
     intro ht
     cases v <;> cases ht <;> grind [ValueTyp, liftValue]
+
+lemma value_typ_ext (ty : Ty) :
+  ValueTyp cCnt defs v ty S → a ∉ S → ValueTyp cCnt defs v ty (S.insert a s) := by
+    intro hv ha
+    unhygienic induction hv <;> try grind [ValueTyp]
+    apply ValueTyp.Cls
+    { rw [Finmap.lookup_insert_of_ne]
+      { exact a_2 }
+      intro heq
+      have st := (Finmap.mem_iff (a := a_1) (s := S_1)).mpr (by
+        eapply Exists.intro
+        solve_by_elim)
+      grind }
+    { grind }
+    grind
+
+lemma loop_jump_delta_ext :
+  LoopJump cCnt defs Δ l → LoopJump cCnt defs (Δ ++ Δ₁) l := by
+    intro hl
+    induction hl <;> grind [LoopJump]
+
+
+theorem lang_extension_delta
+  (tg : Tag) (e : Lang tg) (res : TypR tg)
+  (Γ₁ : Ctx) :
+    Typ cCnt defs tg Δ₁ Γ₁ e res →
+    Typ cCnt defs tg (Δ₁ ++ Δ₂) Γ₁ e res := by
+    intro h
+    unhygienic induction h generalizing Δ₂ <;> try solve_by_elim
+    { apply Typ.FieldAccess <;> solve_by_elim }
+    { apply Typ.Call <;> solve_by_elim }
+    { apply Typ.Return <;> try solve_by_elim
+      { grind }
+      { grind }
+      grind [loop_jump_delta_ext] }
+    apply Typ.BreakExpr
+    induction a <;> solve_by_elim
